final draft for now; so it looks like it didn't actually get pushed and I didn't have time to clean it up :(

pset2/pset2.v
@@ -1,3 +1,5 @@
+(* Jao-ke Chin-Lee *)
+Add LoadPath "/home/jkcl/Dropbox/College/Year4/CS250/jchinlees-cs250-psets/cpdtlib".
 Require Import Bool Arith String List CpdtTactics.
 Require Import FunctionalExtensionality.
 Open Scope string_scope.
@@ -88,18 +90,270 @@ Inductive eval_com : com -> state -> state -> Prop :=
    then you should return the resulting state, and if it doesn't
    terminate in that time, you should return None.  
 *)
+Fixpoint ieval_com (fuel:nat) (c:com) (s:state) {struct fuel} : option state :=
+  match fuel with
+    | 0 => None
+    | S n =>
+      match c with
+        | Skip => Some s
+        | Assign x a => let v := eval_aexp a s in Some (set x v s)
+        | Seq c1 c2 =>
+          match ieval_com n c1 s with
+            | None => None
+            | Some s' => ieval_com n c2 s'
+          end
+        | If b c1 c2 =>
+          if eval_bexp b s then ieval_com n c1 s
+          else ieval_com n c2 s
+        | While b c' => (*ieval_com n (If b (Seq c' c) Skip) s*)
+          if eval_bexp b s then ieval_com n (Seq c' c) s
+          else Some s
+      end
+  end.
+
+Lemma seq_intermed : forall fuel c1 c2 s1 s2, ieval_com (S fuel) (Seq c1 c2) s1 = Some s2 ->
+                                              exists s', ieval_com fuel c1 s1 = Some s' /\
+                                                         ieval_com fuel c2 s' = Some s2.
+Proof.
+  intros.
+  simpl in H.
+  remember (ieval_com fuel c1 s1) as x; destruct x; [ exists s | contradict H ]; crush.
+Qed.
+
+Ltac unroll :=
+  match goal with
+    | [ |- ieval_com (S ?X) _ _ = _] =>
+      let y := fresh in let Heqy := fresh in
+      remember X as y eqn:Heqy; simpl ieval_com; rewrite Heqy
+  end.
+
+Lemma ieval_com_plus' : forall fuel c s1 s2, ieval_com (S fuel) c s1 = Some s2 ->
+                                             ieval_com (S (S fuel)) c s1 = Some s2.
+Proof.
+  intro fuel.
+  induction fuel.
+  (* Base case *)
+  intros.
+  inversion H.
+  destruct c.
+  (* Skip *) crush.
+  (* Assign *) crush.
+  (* Seq *) contradict H1. crush.
+  (* If *)
+  remember (eval_bexp b s1) as x in H1; destruct x; contradict H1; crush.
+  (* While-T *)
+  remember (eval_bexp b s1) as x in H1; destruct x.
+  contradict H1; crush.
+  (* While-F *)
+  unfold ieval_com; reflexivity.
+  (* Inductive step *)
+  destruct c.  intros.
+  (* Skip *)
+  simpl in *. apply H.
+  (* Assign *)
+  simpl in *. crush.
+  (* Seq *)
+  intros.
+  remember (S (S fuel)) as m.
+  simpl ieval_com.
+  remember (ieval_com m c1 s1) as x; destruct x.
+  specialize seq_intermed with (fuel:=(S fuel)) (c1:=c1) (c2:=c2) (s1:=s1) (s2:=s2).
+  intros.
+  rewrite Heqm in H. apply H0 in H. clear H0.
+  destruct H.
+  destruct H.
+  assert (IHfuel1:=IHfuel).
+  specialize IHfuel1 with (c:=c1) (s1:=s1) (s2:=x).
+  apply IHfuel1 in H. clear IHfuel1.
+  assert (IHfuel2:=IHfuel).
+  specialize IHfuel2 with (c:=c2) (s1:=x) (s2:=s2).
+  apply IHfuel2 in H0. clear IHfuel2.
+  rewrite <- Heqx in H.
+  injection H.
+  intros.
+  rewrite H1. apply H0.
+  remember (S fuel) as m'. rewrite Heqm in H.
+  simpl ieval_com in H.
+  remember (ieval_com m' c1 s1) as x; destruct x.
+  assert (IHfuel1:=IHfuel).
+  specialize IHfuel1 with (c:=c1) (s1:=s1) (s2:=s).
+  apply eq_sym in Heqx0. apply IHfuel1 in Heqx0. clear IHfuel1.
+  apply eq_sym in Heqx. contradict Heqx. crush. apply H.
+  (* If *)
+  intros.
+  remember (S (S fuel)) as m.
+  simpl ieval_com.
+  remember (eval_bexp b s1) as x; destruct x;
+  remember (S fuel) as m'; rewrite Heqm in H;
+  simpl ieval_com in H; rewrite <- Heqx in H; assert (IHfuel1:=IHfuel);
+  [ specialize IHfuel1 with (c:=c1) (s1:=s1) (s2:=s2)
+  | specialize IHfuel1 with (c:=c2) (s1:=s1) (s2:=s2) ];
+  apply IHfuel1 in H; apply H.
+  (* While *)
+  intros.
+  remember (S fuel) as m.
+  simpl ieval_com in H.
+  remember (eval_bexp b s1) as x; destruct x.
+  remember (Seq c (While b c)) as c'; destruct c'.
+  crush. crush.
+  unroll.
+  rewrite <- Heqx.
+  rewrite Heqc' in H.
+  assert (IHfuel1:=IHfuel).
+  specialize IHfuel1 with (c:=(Seq c (While b c))) (s1:=s1) (s2:=s2).
+  apply IHfuel1 in H. clear IHfuel1.
+  rewrite H1 in H.
+  apply H.
+  contradict Heqc'. crush.
+  contradict Heqc'. crush.
+  unroll.
+  rewrite <- Heqx.
+  apply H.
+Qed.
+
+Lemma ieval_com_plus : forall fuel c s1 s2, ieval_com fuel c s1 = Some s2 ->
+                                            forall more, ieval_com (fuel+more) c s1 = Some s2.
+Proof.
+  induction fuel.
+  crush.
+  intros.
+  induction more.
+  rewrite plus_comm.
+  crush.
+  rewrite NPeano.Nat.add_succ_r.
+  specialize ieval_com_plus' with (fuel:=(fuel + more)) (c:=c) (s1:=s1) (s2:=s2).
+  intros.
+  apply H0 in IHmore. assumption.
+Qed.
 
 (* Prove that :
 
    eval_com c s1 s2 -> exists n, ieval_com n c s1 = Some s2.
 
 *)
+Theorem if_eval_then_fuel : forall c s1 s2, eval_com c s1 s2 ->
+                                            exists n, ieval_com n c s1 = Some s2.
+Proof.
+  intros.
+  induction H.
+  (* Skip *)
+  exists 1. crush.
+  (* Assign *)
+  exists 1. crush.
+  (* Seq *)
+  destruct IHeval_com1. destruct IHeval_com2.
+  specialize ieval_com_plus with (fuel:=x) (c:=c1) (s1:=s0) (s2:=s1).
+  intros. crush. specialize H4 with (more:=x0).
+  specialize ieval_com_plus with (fuel:=x0) (c:=c2) (s1:=s1) (s2:=s2).
+  intros. crush. specialize H5 with (more:=x).
+  rewrite plus_comm in H4.
+  exists (S (x0+x)).
+  simpl ieval_com. crush.
+  (* If-T *)
+  destruct IHeval_com.
+  exists (S x).
+  simpl ieval_com; crush.
+  (* If-F *)
+  destruct IHeval_com.
+  exists (S x).
+  simpl ieval_com. crush.
+  (* While-F *)
+  exists 1. crush.
+  (* While-T *)
+  destruct IHeval_com1. destruct IHeval_com2.
+  specialize ieval_com_plus with (fuel:=x) (c:=c) (s1:=s1) (s2:=s2).
+  intros. crush. specialize H5 with (more:=x0).
+  specialize ieval_com_plus with (fuel:=x0) (c:=(While b c)) (s1:=s2) (s2:=s3).
+  intros. crush. specialize H6 with (more:=x).
+  rewrite plus_comm in H5.
+  exists (S (S (x0+x))).
+  simpl ieval_com.
+  crush.
+Qed.
 
-(* Prove that : 
-
-   ieval_com n c s1 = Some s2 -> eval_com c s1 s2
-
-*)
+Theorem if_fuel_then_eval : forall n c s1 s2, ieval_com n c s1 = Some s2 ->
+                                              eval_com c s1 s2.
+Proof.
+  Lemma if_fuel_then_eval' : forall n c s1 s2, ieval_com (S n) c s1 = Some s2 ->
+                                               eval_com c s1 s2.
+    Proof.
+      induction n.
+      intros.
+      destruct c.
+      crush. constructor.
+      crush. constructor.
+      crush.
+      crush.
+      (* If *)
+      remember (eval_bexp b s1) as x; destruct x; contradict H; crush.
+      (* While *)
+      crush.
+      remember (eval_bexp b s1) as x; destruct x.
+      contradict H. crush.
+      injection H. intros. clear H.
+      rewrite H0.
+      apply eq_sym in Heqx.
+      constructor. crush.
+      intros.
+      destruct c.
+      crush.
+      crush.
+      (* Seq *)
+      remember (S n) as m.
+      simpl in H.
+      remember (ieval_com m c1 s1) as x; destruct x.
+      apply eq_sym in Heqx.
+      assert (IHn1:=IHn). assert (IHn2:=IHn).
+      specialize IHn1 with (c:=c1) (s1:=s1) (s2:=s).
+      specialize IHn2 with (c:=c2) (s1:=s) (s2:=s2).
+      apply IHn1 in Heqx. clear IHn1.
+      apply IHn2 in H. clear IHn2.
+      apply Eval_seq with (c1:=c1) (s0:=s1) (s1:=s) (c2:=c2) (s2:=s2).
+      crush. apply H.
+      contradict H. crush.
+      (* If-T *)
+      remember (S n) as m.
+      simpl in H.
+      remember (eval_bexp b s1) as x; destruct x.
+      apply eq_sym in Heqx.
+      constructor. apply Heqx. crush.
+      (* If-F *)
+      apply eq_sym in Heqx.
+      apply Eval_if_false with (b:=b) (c1:=c1) (c2:=c2) (s:=s1) (s':=s2).
+      apply Heqx. crush.
+      (* While-T *)
+      remember (S n) as m.
+      simpl in H.
+      remember (eval_bexp b s1) as x; destruct x.
+      apply eq_sym in Heqx.
+      specialize seq_intermed with (fuel:=m) (c1:=c) (c2:=(While b c)) (s1:=s1) (s2:=s2).
+      intros.
+      specialize ieval_com_plus with (fuel:=m) (c:=(Seq c (While b c))) (s1:=s1) (s2:=s2).
+      intros.
+      apply H1 with (more:=1) in H. clear H1.
+      rewrite plus_comm in *.
+      apply H0 in H. clear H0.
+      destruct H.
+      destruct H.
+      assert (IHn1:=IHn). assert (IHn2:=IHn).
+      specialize IHn1 with (c:=c) (s1:=s1) (s2:=x).
+      apply IHn1 in H. clear IHn1.
+      specialize IHn2 with (c:=(While b c)) (s1:=x) (s2:=s2).
+      apply IHn2 in H0. clear IHn2.
+      apply Eval_while_true with (b:=b) (c:=c) (s1:=s1) (s2:=x) (s3:=s2).
+      apply Heqx. apply H. apply H0.
+      (* While-F *)
+      apply eq_sym in Heqx.
+      injection H.
+      intros. clear H.
+      rewrite <- H0.
+      constructor. apply Heqx.
+    Qed.
+    Show.
+    destruct n.
+    intros. simpl in H. crush.
+    apply if_fuel_then_eval'.
+Qed.
 
 (* Write a function
 
@@ -123,6 +377,99 @@ Inductive eval_com : com -> state -> state -> Prop :=
    * replace (if Tt c1 else c2) with c1
    * replace (if Ff c1 else c2) with c2
 *)
+Fixpoint optimize_aexp (a:aexp) : aexp :=
+  match a with
+    | Binop a1 op a2 =>
+      let (a1', a2') := (optimize_aexp a1, optimize_aexp a2) in
+      match op with
+        | Minus => match a2' with Const 0 => a1' | _ => Binop a1' Minus a2' end
+        | Plus =>
+          match (a1', a2') with
+            | (Const 0, _) => a2'
+            | (_, Const 0) => a1'
+            | (_, _) => Binop a1' Plus a2'
+          end
+        | Times =>
+          match (a1', a2') with
+            | (Const 0, _) => Const 0
+            | (Const 1, _) => a2'
+            | (_, Const 0) => Const 0
+            | (_, Const 1) => a1'
+            | (_, _) => Binop a1' Times a2'
+          end
+      end
+    | _ => a
+  end.
+
+Definition eq_aexp_dec (a1 a2:aexp) : {a1=a2} + {a1<>a2}.
+  decide equality.
+  apply (eq_nat_dec n n0).
+  apply (string_dec v v0).
+  decide equality.
+Defined.
+
+Fixpoint optimize_bexp (b:bexp) : bexp :=
+  match b with
+    | Eq a1 a2 =>
+      let (a1', a2') := (optimize_aexp a1, optimize_aexp a2) in
+      match eq_aexp_dec a1' a2' with
+        | left _ => Tt
+        | right _ => Eq a1' a2'
+      end
+    | Lt a1 a2 =>
+      let (a1', a2') := (optimize_aexp a1, optimize_aexp a2) in
+      match eq_aexp_dec a1' a2' with
+        | left _ => Ff
+        | right _ => Lt a1' a2'
+      end
+    | And b1 b2 =>
+      let (b1', b2') := (optimize_bexp b1, optimize_bexp b2) in
+      match (b1', b2') with
+        | (Tt, Tt) => Tt
+        | (Tt, Ff) | (Ff, Tt) | (Ff, Ff) => Ff
+        | _ => And b1' b2'
+      end
+    | Or b1 b2 =>
+      let (b1', b2') := (optimize_bexp b1, optimize_bexp b2) in
+      match (b1', b2') with
+        | (Tt, _) | (_, Tt) => Tt
+        | (Ff, Ff) => Ff
+        | _ => Or b1' b2'
+      end
+    | Not b' =>
+      let b'' := optimize_bexp b' in
+      match b' with
+        | Tt => Ff
+        | Ff => Tt
+        | _ => Not b''
+      end
+    | _ => b
+  end.
+
+Fixpoint optimize_com (c:com) : com :=
+  match c with
+    | Skip => Skip
+    | Assign x a => Assign x (optimize_aexp a)
+    | Seq c1 c2 =>
+      let (c1', c2') := (optimize_com c1, optimize_com c2) in
+      match c1' with
+        | Skip => c2'
+        | _ => match c2' with Skip => c1' | _ => Seq c1' c2' end
+      end
+    | If b c1 c2 =>
+      let b' := optimize_bexp b in
+      match b' with
+        | Tt => optimize_com c1
+        | Ff => optimize_com c2
+        | _ => If b' (optimize_com c1) (optimize_com c2)
+      end
+    | While b c' =>
+      let b' := optimize_bexp b in
+      match b' with
+        | Ff => Skip
+        | _ => While b' (optimize_com c')
+      end
+  end.
 
 (* Construct a proof that optimizing a program doesn't change its
    input/output behavior.  That is, show that if we start in state
@@ -130,7 +477,314 @@ Inductive eval_com : com -> state -> state -> Prop :=
    optimize_com(c) in state s1, we get out a state that is
    extensionally equivalent to s2.  
 *)
-    
+
+Lemma aopt_ok : forall e s, eval_aexp e s = eval_aexp (optimize_aexp e) s.
+Proof.
+  induction e; intros; [ crush | crush | .. ]. (*;
+
+  specialize IHe1 with (s:=s); specialize IHe2 with (s:=s);
+  simpl optimize_aexp; destruct b; simpl;
+  remember (optimize_aexp e1) as e1'; destruct e1';
+  [ destruct n; rewrite IHe1; rewrite IHe2; simpl; crush
+  | remember (optimize_aexp e2) as e2'; destruct e2'
+  | .. ].*)
+
+  simpl optimize_aexp; destruct b; simpl.
+  remember (optimize_aexp e1) as e1'; destruct e1'; specialize IHe1 with (s:=s); specialize IHe2 with (s:=s).
+
+  destruct n. rewrite IHe1. rewrite <- IHe2. simpl. crush. (* or reflexivity instead of crush *)
+  remember (optimize_aexp e2) as e2'; destruct e2'.
+  destruct n0. rewrite <- IHe1. rewrite IHe2. simpl. crush.
+  simpl eval_aexp in *. rewrite IHe1. rewrite IHe2. omega.
+  simpl eval_aexp in *. rewrite IHe1. rewrite IHe2. omega.
+  simpl eval_aexp in *. rewrite IHe1. rewrite IHe2. omega.
+  
+  remember (optimize_aexp e2) as e2'; destruct e2'.
+  destruct n. rewrite IHe1. rewrite IHe2. simpl. omega.
+  simpl eval_aexp in *. rewrite IHe1. rewrite IHe2. omega.
+  simpl eval_aexp in *. rewrite IHe1. rewrite IHe2. omega.
+  simpl eval_aexp in *. rewrite IHe1. rewrite IHe2. omega.
+
+  remember (optimize_aexp e2) as e2'; destruct e2'.
+  destruct n. rewrite IHe1. rewrite IHe2. simpl. omega.
+  simpl eval_aexp in *. rewrite IHe1. rewrite IHe2. simpl. omega.
+  simpl eval_aexp in *. rewrite IHe1. rewrite IHe2. simpl. omega.
+  simpl eval_aexp in *. rewrite IHe1. rewrite IHe2. simpl. omega.
+
+  remember (optimize_aexp e1) as e1'; destruct e1'; specialize IHe1 with (s:=s); specialize IHe2 with (s:=s).
+
+  destruct n. rewrite IHe1. simpl. crush. (* or reflexivity instead of crush *)
+  remember (optimize_aexp e2) as e2'; destruct e2'.
+  destruct n. rewrite IHe1. rewrite IHe2. simpl. omega.
+  destruct n0. rewrite IHe1. rewrite IHe2. simpl. omega.
+  destruct n0. rewrite IHe1. rewrite IHe2. simpl. omega.
+
+  simpl eval_aexp in *. rewrite IHe1. rewrite IHe2. crush.
+  destruct n. rewrite IHe1. rewrite IHe2. simpl. omega.
+  simpl eval_aexp in *. rewrite IHe1. rewrite IHe2. crush.
+  destruct n. rewrite IHe1. rewrite IHe2. simpl. omega.
+  simpl eval_aexp in *. rewrite IHe1. rewrite IHe2. simpl. omega.
+
+  remember (optimize_aexp e2) as e2'; destruct e2'.
+  destruct n. rewrite IHe1. rewrite IHe2. simpl. omega.
+  destruct n. rewrite IHe1. rewrite IHe2. simpl. omega.
+
+  simpl eval_aexp in *. rewrite IHe1. rewrite IHe2. omega.
+  simpl eval_aexp in *. rewrite IHe1. rewrite IHe2. omega.
+  simpl eval_aexp in *. rewrite IHe1. rewrite IHe2. omega.
+  
+  remember (optimize_aexp e2) as e2'; destruct e2'.
+  destruct n. rewrite IHe1. rewrite IHe2. simpl. omega.
+  destruct n. rewrite IHe1. rewrite IHe2. simpl. omega.
+
+  simpl eval_aexp in *. rewrite IHe1. rewrite IHe2. reflexivity.
+  simpl eval_aexp in *. rewrite IHe1. rewrite IHe2. reflexivity.
+  simpl eval_aexp in *. rewrite IHe1. rewrite IHe2. reflexivity.
+
+  remember (optimize_aexp e2) as e2'; destruct e2'; specialize IHe1 with (s:=s); specialize IHe2 with (s:=s).
+  destruct n;
+  simpl eval_aexp in *. rewrite IHe1. rewrite IHe2. simpl. omega.
+  simpl eval_aexp in *. rewrite IHe1. rewrite IHe2. simpl. omega.
+  simpl eval_aexp in *. rewrite IHe1. rewrite IHe2. simpl. omega.
+  simpl eval_aexp in *. rewrite IHe1. rewrite IHe2. simpl. omega.
+Qed.
+
+Lemma my_eq_refl : forall n, NPeano.Nat.eqb n n = true.
+Proof.
+  induction n; crush.
+Qed.
+
+Lemma not_lt_refl : forall n, NPeano.Nat.ltb n n = false.
+Proof.
+  induction n; crush.
+Qed.
+
+Lemma bopt_ok : forall e s, eval_bexp e s = eval_bexp (optimize_bexp e) s.
+Proof.
+  intros; induction e; crush;
+  try ( (* embedded aexps *)
+      remember (eq_aexp_dec (optimize_aexp a) (optimize_aexp a0)) as comp; destruct comp; simpl;
+      specialize aopt_ok with (e:=a) (s:=s); specialize aopt_ok with (e:=a0) (s:=s); intros;
+      rewrite H; rewrite H0;
+      try rewrite e in *;
+        solve
+          [ apply my_eq_refl | apply not_lt_refl | reflexivity ]);
+  try ( (* embedded bexps *)
+      remember (optimize_bexp e1) as e1'; destruct e1'; remember (optimize_bexp e2) as e2'; destruct e2'; simpl; crush).
+  destruct e; simpl; crush.
+Qed.
+
+Ltac remember_cond name :=
+  match goal with
+    | [ |- context[ (If ?c _ _)] ] => remember c as name
+    | [ |- context[ (While ?c _) ] ] => remember c as name
+  end.
+Ltac remember_seq c1name c2name:=
+  match goal with
+    | [ |- context[ (Seq ?c1 ?c2) ] ] => remember c1 as c1name; remember c2 as c2name
+  end.
+
+Theorem opt_ok : forall c s1 s2, eval_com c s1 s2 -> eval_com (optimize_com c) s1 s2.
+Proof.
+  intros.
+  induction H.
+  (* Skip *)
+  simpl. constructor.
+  (* Assign *)
+  simpl optimize_com.
+  specialize aopt_ok with (e:=e) (s:=s). intros.
+  rewrite H.
+  apply Eval_assign with (s:=s) (x:=x) (e:=(optimize_aexp e)).
+  (* Seq *)
+  simpl optimize_com.
+  remember (optimize_com c1) as x; destruct x;
+  [ inversion IHeval_com1; assumption | .. ]; try (
+  remember (optimize_com c2) as y; destruct y;
+  [ inversion IHeval_com2; rewrite <- H3; apply IHeval_com1 | .. ];
+  remember_seq c1' c2'; apply Eval_seq with (c1:=c1') (s0:=s0) (s1:=s1) (c2:=c2') (s2:=s2);
+  solve [ apply IHeval_com1 | apply IHeval_com2]).
+  (* If-T *)
+  simpl optimize_com.
+  remember (optimize_bexp b) as b'; destruct b';
+  [  assumption
+   | apply eq_sym in Heqb';
+     specialize bopt_ok with (e:=b) (s:=s); intros;
+     rewrite H in H1;
+     assert (eval_bexp (optimize_bexp b) s = false);
+     crush | .. ];
+  remember_cond bnew; apply Eval_if_true with (b:=bnew) (c1:=(optimize_com c1)) (c2:=(optimize_com c2)) (s:=s) (s':=s');
+  specialize bopt_ok with (e:=b) (s:=s); intro H1;
+  rewrite H in H1; apply eq_sym in Heqb'; crush;
+  assumption; assumption.
+  (* If-F *)
+  simpl optimize_com.
+  remember (optimize_bexp b) as b'; destruct b';
+  [  apply eq_sym in Heqb';
+     specialize bopt_ok with (e:=b) (s:=s); intros;
+     rewrite H in H1;
+     assert (eval_bexp (optimize_bexp b) s = true);
+     crush
+   | assumption | .. ];
+  remember_cond bnew; apply Eval_if_false with (b:=bnew) (c1:=(optimize_com c1)) (c2:=(optimize_com c2)) (s:=s) (s':=s');
+  specialize bopt_ok with (e:=b) (s:=s); intro H1;
+  rewrite H in H1; apply eq_sym in Heqb'; crush;
+  assumption; assumption.
+  (* While-F *)
+  Lemma static_true : forall b, optimize_bexp b = Tt -> (forall s, eval_bexp b s = true).
+  Proof.
+    intros. rewrite bopt_ok. rewrite H. crush.
+  Qed.
+
+  Lemma no_inf_ieval : forall n c s, ieval_com n (While Tt c) s = None /\ ieval_com (S n) (While Tt c) s = None.
+  Proof.
+    induction n.
+    crush.
+    intros.
+    assert (IHn1:=IHn). assert (IHn2:=IHn).
+    specialize IHn1 with (c:=c) (s:=s).
+    destruct IHn1. split. assumption.
+    simpl ieval_com.
+    remember (ieval_com n c s) as x; destruct x.
+    specialize IHn2 with (c:=c) (s:=s0).
+    destruct IHn2. assumption.
+    crush.
+  Qed.
+  Lemma no_inf_eval : forall c s1 s2, eval_com (While Tt c) s1 s2 -> False.
+  Proof.
+    intros.
+    specialize if_eval_then_fuel with (c:=(While Tt c)) (s1:=s1) (s2:=s2).
+    specialize no_inf_ieval with (c:=(While Tt c)) (s:=s1).
+    intros.
+    destruct H1. assumption.
+    specialize if_fuel_then_eval with (n:=x) (c:=(While Tt c)) (s1:=s1) (s2:=s2).
+    specialize H0 with (n:=x) (c:=c) (s:=s1).
+    destruct H0.
+    contradict H1. crush.
+  Qed.
+
+  simpl optimize_com.
+  remember (optimize_bexp b) as b'; destruct b';
+  [ apply eq_sym in Heqb';
+    specialize bopt_ok with (e:=b) (s:=s); intros;
+    rewrite H in H0;
+    assert (eval_bexp (optimize_bexp b) s = true);
+    crush;
+    apply eq_sym in H0; contradict H1; discriminate
+  | apply Eval_skip with (s:=s) | .. ];
+  remember_cond b'';
+  apply Eval_while_false with (b:=b'') (c:=(optimize_com c)) (s:=s);
+  specialize bopt_ok with (e:=b) (s:=s); intro Hopt_eq;
+  rewrite H in Hopt_eq; rewrite <- Heqb' in Hopt_eq;
+  apply eq_sym in Hopt_eq; assumption.
+  (* While-T *)
+  simpl optimize_com.
+  remember (optimize_bexp b) as b'; destruct b'.
+  apply Eval_while_true with (b:=Tt) (c:=(optimize_com c)) (s1:=s1) (s2:=s2) (s3:=s3).
+  crush.
+  assumption.
+  apply eq_sym in Heqb'.
+  eapply if_eval_then_fuel in IHeval_com2.
+  destruct IHeval_com2.
+  assert (exists x1, x = S x1).
+  induction x. contradict H2. crush. exists x. reflexivity.
+  destruct H3.
+  simpl in H2. 
+  rewrite Heqb' in H2.
+  pose proof no_inf_ieval.
+  contradict H2.
+  specialize H4 with (n:=x) (c:=(optimize_com c)) (s:=s2).
+  destruct H4.
+  rewrite H2. discriminate.
+
+  specialize bopt_ok with (e:=b) (s:=s1). intros.
+  rewrite <- Heqb' in H2. simpl in H2. contradict H. crush.
+
+  remember_cond b'.
+  apply Eval_while_true with (b:=b') (c:=(optimize_com c)) (s1:=s1) (s2:=s2) (s3:=s3).
+  specialize bopt_ok with (e:=b) (s:=s1). intro Hopt_eq.
+  rewrite H in Hopt_eq. rewrite <- Heqb' in Hopt_eq.
+  apply eq_sym in Hopt_eq; assumption.
+  assumption.
+  eapply if_eval_then_fuel in IHeval_com2.
+  destruct IHeval_com2.
+  assert (exists x1, x = S x1).
+  induction x. contradict H2. crush. exists x. reflexivity.
+  destruct H3.
+  simpl in H2.
+  rewrite <- Heqb' in H2.
+  rewrite Heqb'0 in H2.
+  eapply if_fuel_then_eval with (n:=x).
+  rewrite Heqb'0. assumption.
+  remember_cond b'.
+  apply Eval_while_true with (b:=b') (c:=(optimize_com c)) (s1:=s1) (s2:=s2) (s3:=s3).
+  specialize bopt_ok with (e:=b) (s:=s1). intro Hopt_eq.
+  rewrite H in Hopt_eq. rewrite <- Heqb' in Hopt_eq.
+  apply eq_sym in Hopt_eq; assumption.
+  assumption.
+  eapply if_eval_then_fuel in IHeval_com2.
+  destruct IHeval_com2.
+  assert (exists x1, x = S x1).
+  induction x. contradict H2. crush. exists x. reflexivity.
+  destruct H3.
+  simpl in H2.
+  rewrite <- Heqb' in H2.
+  rewrite Heqb'0 in H2.
+  eapply if_fuel_then_eval with (n:=x).
+  rewrite Heqb'0. assumption.
+
+  remember_cond b'.
+  apply Eval_while_true with (b:=b') (c:=(optimize_com c)) (s1:=s1) (s2:=s2) (s3:=s3).
+  specialize bopt_ok with (e:=b) (s:=s1). intro Hopt_eq.
+  rewrite H in Hopt_eq. rewrite <- Heqb' in Hopt_eq.
+  apply eq_sym in Hopt_eq; assumption.
+  assumption.
+  eapply if_eval_then_fuel in IHeval_com2.
+  destruct IHeval_com2.
+  assert (exists x1, x = S x1).
+  induction x. contradict H2. crush. exists x. reflexivity.
+  destruct H3.
+  simpl in H2.
+  rewrite <- Heqb' in H2.
+  rewrite Heqb'0 in H2.
+  eapply if_fuel_then_eval with (n:=x).
+  rewrite Heqb'0. assumption.
+
+
+  remember_cond b'.
+  apply Eval_while_true with (b:=b') (c:=(optimize_com c)) (s1:=s1) (s2:=s2) (s3:=s3).
+  specialize bopt_ok with (e:=b) (s:=s1). intro Hopt_eq.
+  rewrite H in Hopt_eq. rewrite <- Heqb' in Hopt_eq.
+  apply eq_sym in Hopt_eq; assumption.
+  assumption.
+  eapply if_eval_then_fuel in IHeval_com2.
+  destruct IHeval_com2.
+  assert (exists x1, x = S x1).
+  induction x. contradict H2. crush. exists x. reflexivity.
+  destruct H3.
+  simpl in H2.
+  rewrite <- Heqb' in H2.
+  rewrite Heqb'0 in H2.
+  eapply if_fuel_then_eval with (n:=x).
+  rewrite Heqb'0. assumption.
+
+
+  remember_cond b''.
+  apply Eval_while_true with (b:=b'') (c:=(optimize_com c)) (s1:=s1) (s2:=s2) (s3:=s3).
+  specialize bopt_ok with (e:=b) (s:=s1). intro Hopt_eq.
+  rewrite H in Hopt_eq. rewrite <- Heqb' in Hopt_eq.
+  apply eq_sym in Hopt_eq; assumption.
+  assumption.
+  eapply if_eval_then_fuel in IHeval_com2.
+  destruct IHeval_com2.
+  assert (exists x1, x = S x1).
+  induction x. contradict H2. crush. exists x. reflexivity.
+  destruct H3.
+  simpl in H2.
+  rewrite <- Heqb' in H2.
+  rewrite Heqb'' in H2.
+  eapply if_fuel_then_eval with (n:=x).
+  rewrite Heqb''. assumption.
+Qed.
 
 
 (* Hints:
